Discretion/Monad/Ordered.lean
@@ -1,4 +1,5 @@
 import Discretion.Order.Discrete
+import Mathlib.Data.Set.Functor
 
 instance Disc.instMonad : Monad Disc := Id.instMonad
 
@@ -12,14 +13,74 @@ instance DiscBot.instMonad : Monad DiscBot := (inferInstance : Monad Option)
 
 instance DiscBot.instLawfulMonad : LawfulMonad DiscBot := (inferInstance : LawfulMonad Option)
 
+-- TODO: DiscBounded is also a LawfulMonad
+
+@[simp]
+theorem DiscTop.bind_top {α β} (f : α → DiscTop β) : ⊤ >>= f = ⊤ := rfl
+
+@[simp]
+theorem DiscTop.bind_some {α β} (a : α) (f : α → DiscTop β) : some a >>= f = f a := rfl
+
+@[simp]
+theorem DiscTop.bind_coe {α β} (a : α) (f : α → DiscTop β) : a >>= f = f a := rfl
+
+@[simp]
+theorem DiscBot.bind_bot {α β} (f : α → DiscBot β) : ⊥ >>= f = ⊥ := rfl
+
+@[simp]
+theorem DiscBot.bind_some {α β} (a : α) (f : α → DiscBot β) : some a >>= f = f a := rfl
+
+@[simp]
+theorem DiscBot.bind_coe {α β} (a : α) (f : α → DiscBot β) : a >>= f = f a := rfl
+
 class OrderedMonad (m : Type u → Type v) [Monad m] [∀α, LE (m α)] where
   bind_mono {α β} {a a' : m α} {f f' : α → m β} (ha : a ≤ a') (hf : f ≤ f') : a >>= f ≤ a' >>= f'
 
 instance Disc.instOrderedMonad : OrderedMonad Disc where
   bind_mono ha hf := by cases ha; cases (DiscreteOrder.le_eq _ _ hf); rfl
 
--- instance DiscTop.instOrderedMonad : OrderedMonad DiscTop where
---   bind_mono ha hf := sorry
+instance DiscTop.instOrderedMonad : OrderedMonad DiscTop where
+  bind_mono ha hf := by
+    apply DiscTop.leCases (h := ha)
+    · intro a; simp
+    · intro a; simp [hf a]
 
--- instance DiscBot.instOrderedMonad : OrderedMonad DiscBot where
---   bind_mono ha hf := sorry
+instance DiscBot.instOrderedMonad : OrderedMonad DiscBot where
+  bind_mono ha hf := by
+    apply DiscBot.leCases (h := ha)
+    · intro a; simp
+    · intro a; simp [hf a]
+
+-- TODO: DiscBounded is also an OrderedMonad
+
+class TopMonad (m : Type u → Type v) [Monad m] [∀α, Top (m α)] where
+  bind_top {α β} (f : α → m β) : ⊤ >>= f = ⊤
+
+instance DiscTop.instTopMonad : TopMonad DiscTop where
+  bind_top _ := rfl
+
+class BotMonad (m : Type u → Type v) [Monad m] [∀α, Bot (m α)] where
+  bind_bot {α β} (f : α → m β) : ⊥ >>= f = ⊥
+
+instance DiscBot.instBotMonad : BotMonad DiscBot where
+  bind_bot _ := rfl
+
+-- TODO: DiscBounded is a TopMonad and a BotMonad
+
+-- TODO: more interesting:
+-- - the trace monad with an ordered monoid
+-- - the nondeterminism monad
+
+attribute [local instance] Set.monad
+
+instance Set.ordered_monad : OrderedMonad Set where
+  bind_mono ha hf := by
+    simp only [bind_def, le_eq_subset, iUnion_subset_iff]
+    intro a ha' b hb'
+    simp only [mem_iUnion, exists_prop]
+    exact ⟨a, ha ha', hf a hb'⟩
+
+instance Set.bot_monad : BotMonad Set where
+  bind_bot _ := by simp
+
+-- Note: set is _not_ a `TopMonad`, since not every α → Set β is a covering!
